\documentclass{amsart}

\input{preamble}

\title{ISIS1105 - 202520\\ Tarea 2\\ SecciÃ³n 2}
\author{Daniel R. Barrero R.}

\begin{document}
\maketitle

%%
\section{LHRRs - no repeated roots}

%

\subsection{} Solve
\begin{displaymath}
	\begin{cases}
		t(0)= 4\\
		t(n)= -3t(n-1),\ n \geq 1.
	\end{cases}
\end{displaymath}

%

\subsection{} Solve
\begin{displaymath}
	\begin{cases}
		t(0)= 1,\ t(1)= 2\\
		t(n)= -t(n-1) + 6t(n-2),\ n \geq 2.
	\end{cases}
\end{displaymath}

%

\subsection{} Find the recurrence of which
\[
	t(n)= \sqrt{3}(-3)^n - \sqrt{2}2^n
\]
is the unique solution.

%%
\section{LHRRs - repeated roots}
\begin{thm}\label{hrep}
	If the recurrence
	\[
		t(n)= \sum_{i= 1}^k a_i t(n-i)
	\]
	has characteristic equation
	\[
		E(x)(x-c)^d= 0,
	\]
	where $d > 1$ and $c$ is not a solution of $E(x)= 0$, then its solutions
	are of the form
	\[
		t(n) = \xi(n) + u_0c^n + u_1nc^n + \cdots u_{d-1}n^{d-1}c^n,
	\]
	where the $u_i$ are constants and $\xi(n)$ is a solution of the
	recurrence with characteristic equation $E(x)= 0$.
\end{thm}

%

\subsection{} Solve
\[
	\begin{cases}
		t(0)= 0,\ t(1)= -1,\ t(2)= 0,\ t(3)= 1\\
		t(n)= 2t(n-1) + t(n-2) - 2t(n-3) - t(n-4),\ n \geq 4.
	\end{cases}
\]

\textit{[\textbf{Hint}: The characteristic polynomial is divisible by $x^2 - x - 1$.]}

%%
\section{LRRs - inhomogeneous problems}
\begin{thm}
	If the initial value problem
	\begin{displaymath}
		\begin{cases}
			t(0)= v_0, \cdots, t(k-1)= v_{k-1}\\
			t(n)+ \sum_{i= 1}^k b_it(n-i)= q,\ n \geq k
		\end{cases}
	\end{displaymath}
	is such that $q = c^np(n)$, where $c$ is a positive constant and
	$p(n)$ is a polynomial of degree $d$, then it is equivalent to a
	homogeneous problem of degree $k+d+1$ with characteristic equation
	\begin{equation*}
		E(x)(x-c)^{d+1} = 0
	\end{equation*}
	where $E(x) = 0$ is the characteristic equation of
	\[
		t(n) + \sum_{i= 1}^k b_it(n-i)= 0.
	\]
\end{thm}

%

\subsection{} Solve
\[
	\begin{cases}
		t(0)= 0\\
		t(n)= -3t(n-1) + 2^n,\ n\geq 1.
	\end{cases}
\]

%

\subsection{} Solve
\[
	\begin{cases}
		t(0)= 0\\
		t(n)= -3t(n-1) + 2n,\ n\geq 1.
	\end{cases}
\]

\subsection{} Solve
\[
	\begin{cases}
		t(0)= 0\\
		t(n)= -3t(n-1) + (n^2 + 1)2^n,\ n\geq 1.
	\end{cases}
\]
\end{document}
